Bump Iris (persistent mapsto).

theories/concurrent_stacks/concurrent_stack3.v
@@ -26,24 +26,6 @@ Section stack_works.
   Context `{!heapG Σ} (N : namespace).
   Implicit Types l : loc.
 
-  Local Notation "l ↦{-} v" := (∃ q, l ↦{q} v)%I
-    (at level 20, format "l  ↦{-}  v") : bi_scope.
-
-  Lemma partial_mapsto_duplicable l v :
-    l ↦{-} v -∗ l ↦{-} v ∗ l ↦{-} v.
-  Proof.
-    iIntros "H"; iDestruct "H" as (?) "[Hl Hl']"; iSplitL "Hl"; eauto.
-  Qed.
-
-  Lemma partial_mapsto_agree l v1 v2 :
-    l ↦{-} v1 -∗ l ↦{-} v2 -∗ ⌜v1 = v2⌝.
-  Proof.
-    iIntros "H1 H2".
-    iDestruct "H1" as (?) "H1".
-    iDestruct "H2" as (?) "H2".
-    iApply (mapsto_agree with "H1 H2").
-  Qed.
-
   Definition oloc_to_val (ol: option loc) : val :=
     match ol with
     | None => NONEV
@@ -55,20 +37,19 @@ Section stack_works.
   Fixpoint is_list xs v : iProp Σ :=
     (match xs, v with
      | [], None => True
-     | x :: xs, Some l => ∃ t, l ↦{-} (x, oloc_to_val t)%V ∗ is_list xs t
+     | x :: xs, Some l => ∃ t, l ↦□ (x, oloc_to_val t)%V ∗ is_list xs t
      | _, _ => False
      end)%I.
 
   Lemma is_list_dup xs v :
     is_list xs v -∗ is_list xs v ∗ match v with
       | None => True
-      | Some l => ∃ h t, l ↦{-} (h, oloc_to_val t)%V
+      | Some l => ∃ h t, l ↦□ (h, oloc_to_val t)%V
       end.
   Proof.
     destruct xs, v; simpl; auto; first by iIntros "[]".
-    iIntros "H"; iDestruct "H" as (t) "(Hl & Hstack)".
-    iDestruct (partial_mapsto_duplicable with "Hl") as "[Hl1 Hl2]".
-    iSplitR "Hl2"; first by (iExists _; iFrame). by iExists _, _.
+    iIntros "H"; iDestruct "H" as (t) "[#Hl Hstack]".
+    iSplitL; first by (iExists _; iFrame). by iExists _, _.
   Qed.
 
   Lemma is_list_empty xs :
@@ -78,13 +59,13 @@ Section stack_works.
   Qed.
 
   Lemma is_list_cons xs l h t :
-    l ↦{-} (h, t)%V -∗
+    l ↦□ (h, t)%V -∗
     is_list xs (Some l) -∗
     ∃ ys, ⌜xs = h :: ys⌝.
   Proof.
     destruct xs; first by iIntros "? %".
     iIntros "Hl Hstack"; iDestruct "Hstack" as (t') "(Hl' & Hrest)".
-    iDestruct (partial_mapsto_agree with "Hl Hl'") as "%"; simplify_eq; iExists _; auto.
+    iDestruct (mapsto_agree with "Hl Hl'") as "%"; simplify_eq; iExists _; auto.
   Qed.
 
   Definition stack_inv P l :=
@@ -121,8 +102,9 @@ Section stack_works.
     iInv N as (list' xs) "(Hl & Hlist & HP)" "Hclose".
     destruct (decide (list = list')) as [ -> |].
     - wp_cmpxchg_suc. { destruct list'; left; done. }
+      iMod (mapsto_persist with "Hl'") as "#Hl'".
       iMod ("Hupd" with "HP") as "[HP HΨ]".
-      iMod ("Hclose" with "[Hl Hl' HP Hlist]") as "_".
+      iMod ("Hclose" with "[Hl HP Hlist]") as "_".
       { iNext; iExists (Some _), (v :: xs); iFrame; iExists _; iFrame; auto. }
       iModIntro.
       wp_pures.
@@ -166,7 +148,6 @@ Section stack_works.
       iModIntro.
       wp_match. wp_bind (Load _).
       iInv N as (v xs') "(Hl & Hlist & HP)" "Hclose".
-      iDestruct "Hl'" as (q) "Hl'".
       wp_load.
       iMod ("Hclose" with "[Hlist Hl HP]") as "_".
       { iNext; iExists _, _; iFrame. }
@@ -175,12 +156,11 @@ Section stack_works.
       iInv N as (v' xs'') "(Hl & Hlist & HP)" "Hclose".
       destruct (decide (v' = (Some l'))) as [ -> |].
       * wp_cmpxchg_suc.
-        iDestruct (is_list_cons with "[Hl'] Hlist") as (ys) "%"; first by iExists _.
+        iDestruct (is_list_cons with "Hl' Hlist") as (ys) "%".
         simplify_eq.
         iDestruct "Hupd" as "[Hupdcons _]".
         iMod ("Hupdcons" with "HP") as "[HP HΨ]".
         iDestruct "Hlist" as (t') "(Hl'' & Hlist)".
-        iDestruct "Hl''" as (q') "Hl''".
         iDestruct (mapsto_agree with "Hl' Hl''") as "%"; simplify_eq.
         iMod ("Hclose" with "[Hlist Hl HP]") as "_".
         { iNext; iExists _, _; iFrame. }
