theories/logrel/F_mu_ref_conc/examples/stack/stack_rules.v
@@ -1,33 +1,12 @@
 From iris.proofmode Require Import tactics.
-From iris.algebra Require Import auth gmap agree.
 From iris_examples.logrel.F_mu_ref_conc Require Import logrel_binary.
-Import uPred.
-
-Definition stackUR : ucmraT := gmapUR loc (agreeR valO).
-
-Class stackG Σ :=
-  StackG { stack_inG :> inG Σ (authR stackUR); stack_name : gname }.
-
-Definition stack_mapsto `{stackG Σ} (l : loc) (v : val) : iProp Σ :=
-  own stack_name (◯ {[ l := to_agree v ]}).
-
-Notation "l ↦ˢᵗᵏ v" := (stack_mapsto l v) (at level 20) : bi_scope.
 
 Section Rules.
-  Context `{stackG Σ}.
+  Context `{heapIG Σ}.
   Notation D := (prodO valO valO -n> iPropO Σ).
 
-  Global Instance stack_mapsto_persistent l v : Persistent (l ↦ˢᵗᵏ v).
-  Proof. apply _. Qed.
-
-  Lemma stack_mapstos_agree l v w : l ↦ˢᵗᵏ v ∗ l ↦ˢᵗᵏ w ⊢ ⌜v = w⌝.
-  Proof.
-    rewrite -own_op -auth_frag_op singleton_op own_valid.
-    by iIntros (->%auth_frag_valid%singleton_valid%to_agree_op_inv_L).
-  Qed.
-
   Program Definition StackLink_pre (Q : D) : D -n> D := λne P v,
-    (∃ l w, ⌜v.1 = LocV l⌝ ∗ l ↦ˢᵗᵏ w ∗
+    (∃ l w, ⌜v.1 = LocV l⌝ ∗ l ↦ᵢ□ w ∗
             ((⌜w = InjLV UnitV⌝ ∧ ⌜v.2 = FoldV (InjLV UnitV)⌝) ∨
             (∃ y1 z1 y2 z2, ⌜w = InjRV (PairV y1 (FoldV z1))⌝ ∗
               ⌜v.2 = FoldV (InjRV (PairV y2 z2))⌝ ∗ Q (y1, y2) ∗ ▷ P(z1, z2))))%I.
@@ -40,7 +19,7 @@ Section Rules.
 
   Lemma StackLink_unfold Q v :
     StackLink Q v ≡ (∃ l w,
-      ⌜v.1 = LocV l⌝ ∗ l ↦ˢᵗᵏ w ∗
+      ⌜v.1 = LocV l⌝ ∗ l ↦ᵢ□ w ∗
       ((⌜w = InjLV UnitV⌝ ∧ ⌜v.2 = FoldV (InjLV UnitV)⌝) ∨
       (∃ y1 z1 y2 z2, ⌜w = InjRV (PairV y1 (FoldV z1))⌝
                       ∗ ⌜v.2 = FoldV (InjRV (PairV y2 z2))⌝
@@ -57,54 +36,7 @@ Section Rules.
     iDestruct "H" as (l w) "[% [#Hl [#Hr|Hr]]]"; subst.
     { iExists l, w; iModIntro; eauto. }
     iDestruct "Hr" as (y1 z1 y2 z2) "[#H1 [#H2 [#HQ H']]]".
-    rewrite later_forall. iDestruct ("IH" with "H'") as "#H''". iClear "H'".
+    iDestruct ("IH" with "H'") as "#H''". iClear "H'".
     iModIntro. eauto 20.
   Qed.
-
-  Lemma stackR_alloc (h : stackUR) (i : loc) (v : val) :
-    h !! i = None → ● h ~~> ● (<[i := to_agree v]> h) ⋅ ◯ {[i := to_agree v]}.
-  Proof. intros. by apply auth_update_alloc, alloc_singleton_local_update. Qed.
-
-  Context `{heapIG Σ}.
-
-  Definition stack_owns (h : gmap loc val) :=
-    (own stack_name (● ((to_agree <$> h) : stackUR))
-        ∗ [∗ map] l ↦ v ∈ h, l ↦ᵢ v)%I.
-
-  Lemma stack_owns_alloc h l v :
-    stack_owns h ∗ l ↦ᵢ v ==∗ stack_owns (<[l := v]> h) ∗ l ↦ˢᵗᵏ v.
-  Proof.
-    iIntros "[[Hown Hall] Hl]".
-    iDestruct (own_valid with "Hown") as %Hvalid.
-    destruct (h !! l) as [w|] eqn:?.
-    { iDestruct (@big_sepM_lookup with "Hall") as "Hl'"; first done.
-      by iDestruct (@mapsto_valid_2 loc val with "Hl Hl'") as %[??]. }
-    iMod (own_update with "Hown") as "[Hown Hl']".
-    { eapply auth_update_alloc.
-        eapply (alloc_singleton_local_update _ l (to_agree v)); last done.
-    by rewrite lookup_fmap Heqo. }
-    iModIntro. rewrite /stack_owns. rewrite fmap_insert. iFrame "Hl' Hown".
-    iApply @big_sepM_insert; simpl; try iFrame; auto.
-  Qed.
-
-  Lemma stack_owns_open_close h l v :
-    stack_owns h -∗ l ↦ˢᵗᵏ v -∗ l ↦ᵢ v ∗ (l ↦ᵢ v -∗ stack_owns h).
-  Proof.
-    iIntros "[Howns Hls] Hl".
-    iDestruct (own_valid_2 with "Howns Hl")
-      as %[[az [Haz Hq]]%singleton_included_l _]%auth_both_valid_discrete.
-    rewrite lookup_fmap in Haz.
-    assert (∃ z, h !! l = Some z) as Hz.
-    { revert Haz; case: (h !! l) => [z|] Hz; first (by eauto); inversion Hz. }
-    destruct Hz as [z Hz]; rewrite Hz in Haz.
-    apply Some_equiv_inj in Haz; revert Hq; rewrite -Haz => Hq.
-    apply Some_included_total, to_agree_included, leibniz_equiv in Hq; subst.
-    rewrite (big_sepM_lookup_acc _ _ l); eauto.
-    iDestruct "Hls" as "[Hl' Hls]".
-    iIntros "{$Hl'} Hl'". rewrite /stack_owns. iFrame "Howns". by iApply "Hls".
-  Qed.
-
-  Lemma stack_owns_later_open_close h l v :
-    ▷ stack_owns h -∗ l ↦ˢᵗᵏ v -∗ ▷ (l ↦ᵢ v ∗ (l ↦ᵢ v -∗ stack_owns h)).
-  Proof. iIntros "H1 H2". iNext; by iApply (stack_owns_open_close with "H1"). Qed.
 End Rules.
